Separate Compilation and Backtranslation to their own files

rupicola/stlc/RrHP.fst
@@ -5,70 +5,13 @@ open FStar.Tactics.Typeclasses
 
 open STLC
 open QTyp
+open QExp
 open ExpRel
-open Compiler
-
-
-// the environment is non-standard, more fancy
-// also over qType instead of syntactic types (typ)
-noeq type typing : typ_env -> exp -> qType -> Type =
-  | TyUnit : #g:typ_env ->
-             typing g EUnit tunit
-  | TyTrue : #g:typ_env ->
-             typing g ETrue tbool
-  | TyFalse : #g:typ_env ->
-              typing g EFalse tbool
-  | TyIf : #g:typ_env ->
-           #e1:exp ->
-           #e2:exp ->
-           #e3:exp ->
-           #t:qType ->
-           $h1:typing g e1 tbool ->
-           $h2:typing g e2 t ->
-           $h3:typing g e3 t ->
-             typing g (EIf e1 e2 e3) t
-  | TyVar : #g:typ_env ->
-            x:var{Some? (g x)} ->
-              typing g (EVar x) (Some?.v (g x))
-  | TyLam : #g:typ_env ->
-            #body:exp ->
-            #t1:qType ->
-            #t2:qType ->
-            $hbody:typing (extend t1 g) body t2 ->
-              typing g (ELam body) (t1 ^-> t2)
-  | TyApp : #g:typ_env ->
-            #e1:exp ->
-            #e2:exp ->
-            #t1:qType ->
-            #t2:qType ->
-            $h1:typing g e1 (t1 ^-> t2) ->
-            $h2:typing g e2 t1 ->
-              typing g (EApp e1 e2) t2
-  | TyPair : #g:typ_env ->
-            #e1:exp ->
-            #e2:exp ->
-            #t1:qType ->
-            #t2:qType ->
-            $h1:typing g e1 t1 ->
-            $h2:typing g e2 t2 ->
-              typing g (EPair e1 e2) (t1 ^* t2)
-  | TyFst : #g:typ_env ->
-            #e:exp ->
-            #t1:qType ->
-            #t2:qType ->
-            $h1:typing g e (t1 ^* t2) ->
-              typing g (EFst e) t1
-  | TySnd : #g:typ_env ->
-            #e:exp ->
-            #t1:qType ->
-            #t2:qType ->
-            $h1:typing g e (t1 ^* t2) ->
-              typing g (ESnd e) t2
-
+open Compilation
+open Backtranslation
 
 noeq type intS = {
-  ct : Type; // type of context
-  comp_ct : compile_typ ct; // compiled type of context, F* will crash if ct is not a type for which the compile_typ class has an instance
+  ct : qType;
 }
 
 (* CA: this definition of progS is very comical! I have the compiled program inside the guarantee that it can be compiled :D **)
@@ -76,8 +19,12 @@ noeq type intS = {
 // program is dependent pair type with:
   // map from the type of context to bool (which represents output of the source program)
   // (proof of) compiled closed expression - where we pass in the type of ps (#_), the (proof of the) type of the compiled closed expression (#(compile_typ_arrow ...)), and ps
-type progS (i:intS) = ps:(i.ct -> bool) & compile_closed #_ #(compile_typ_arrow _ bool #i.comp_ct) ps
-type ctxS (i:intS) = i.ct
+type progS (i:intS) =
+  ps:(get_Type i.ct -> bool)
+  &
+  exp_quotation #(i.ct ^-> qBool) empty (fun _ -> ps)
+
+type ctxS (i:intS) = get_Type i.ct
 type wholeS = bool // CA: To be able to compile whole programs requires a proof that it can be compiled
 
 // linking involves taking a program and context, extracting the first part of the dependent pair (so the program i.ct -> bool) and applying it to the context
@@ -96,14 +43,14 @@ let behS ws = ws
 noeq type intT = { ct : qType }
 
 val comp_int : intS -> intT
-let comp_int i = { ct = pack i.comp_ct }
+//let comp_int i = { ct = type_quotation_to_typ i.qct }
+let comp_int i = { ct = i.ct }
 
 type progT (i:intT) = closed_exp
 
 // the typing makes sure that there are no pre post conditions - maybe...
 type ctxT (i:intT) = ct:value & typing empty ct i.ct
-(** CA: syntactic typing necessary so that one can backtranslate and to know the type.
-   **)
+(** syntactic typing necessary to be able to backtranslate **)
 type wholeT = closed_exp
 
 let linkT (#i:intT) (pt:progT i) (ct:ctxT i) : wholeT =
@@ -112,7 +59,7 @@ let linkT (#i:intT) (pt:progT i) (ct:ctxT i) : wholeT =
   wt
 
 let compile_prog (#i:intS) (ps:progS i) : progT (comp_int i) =
-  (dsnd ps).e
+  compile_closed (dsnd ps)
 
 let rel_bools (fs_e:bool) (e:exp) : Type0 =
   (e == ETrue /\ fs_e == true) \/
@@ -137,169 +84,44 @@ let lem_rel_beh (fs_e:wholeS) (e:wholeT)
 
 (** ** Proof of RrHP **)
 
-let rec exp_to_fstar (g:typ_env) (e:exp) (t:qType) (h:typing g e t) (fs_g:eval_env g) : (get_Type t) =
-  match e with
-  | EUnit -> ()
-  | ETrue -> true
-  | EFalse -> false
-  | EIf e1 e2 e3 ->
-    let TyIf #_ #_ #_ #_ #t h1 h2 h3 = h in
-    let b : bool = exp_to_fstar g e1 tbool h1 fs_g in
-    let v1 = exp_to_fstar g e2 t h2 fs_g in
-    let v2 = exp_to_fstar g e3 t h3 fs_g in
-    if b then v1 else v2
-  | EVar x -> index fs_g x
-  | ELam body ->
-    let TyLam #_ #_ #t1 #t2 hbody = h in
-    assert (t == (t1 ^-> t2));
-    let w : (get_Type t1) -> (get_Type t2) =
-      (fun x -> exp_to_fstar (extend t1 g) body t2 hbody (stack fs_g x)) in
-    w
-  | EApp e1 e2 ->
-    let TyApp #_ #_ #_ #t1 #t2 h1 h2 = h in
-    assert ((get_Type t) == (get_Type t2));
-    let v1 : get_Type (t1 ^-> t2) = exp_to_fstar g e1 (t1 ^-> t2) h1 fs_g in
-    let v2 : get_Type t1 = exp_to_fstar g e2 t1 h2 fs_g in
-    v1 v2
-  | EPair e1 e2 ->
-    let TyPair #_ #_ #_ #t1 #t2 h1 h2 = h in
-    let v1 = exp_to_fstar g e1 t1 h1 fs_g in
-    let v2 = exp_to_fstar g e2 t2 h2 fs_g in
-    (v1, v2)
-  | EFst e ->
-    let TyFst #_ #_ #t1 #t2 h1 = h in
-    let v = exp_to_fstar g e (t1 ^* t2) h1 fs_g in
-    fst #(get_Type t1) #(get_Type t2) v
-  | ESnd e ->
-    let TySnd #_ #_ #t1 #t2 h1 = h in
-    let v = exp_to_fstar g e (t1 ^* t2) h1 fs_g in
-    snd #(get_Type t1) #(get_Type t2) v
-
 val backtranslate_ctx : (#i:intS) -> ctxT (comp_int i) -> ctxS i
 let backtranslate_ctx (#i:intS) (ctxt:ctxT (comp_int i)) : ctxS i =
   let (| e, h |) = ctxt in
-  exp_to_fstar empty e (comp_int i).ct h empty_eval
+  backtranslate empty e (comp_int i).ct h empty_eval
 
-#push-options "--split_queries always"
-val lem_exp_to_fstar g (e:exp{fv_in_env g e}) t (h:typing g e t) : Lemma
-(equiv t (exp_to_fstar g e t h) e)
-let rec lem_exp_to_fstar g e t (h:typing g e t) =
-   match e with
-  | EUnit -> equiv_unit g
-  | ETrue -> equiv_true g
-  | EFalse -> equiv_false g
-  | EVar x -> equiv_var g x
-  | EPair e1 e2 ->
-    let TyPair #_ #_ #_ #t1 #t2 h1 h2 = h in
-    lem_pair_fv_in_env g e1 e2;
-    lem_exp_to_fstar g e1 t1 h1;
-    lem_exp_to_fstar g e2 t2 h2;
-    let fs_e1 = (exp_to_fstar g e1 t1 h1) in
-    let fs_e2 = (exp_to_fstar g e2 t2 h2) in
-    equiv_pair g t1 t2 fs_e1 fs_e2 e1 e2
-  | EIf e1 e2 e3 ->
-    let TyIf #_ #_ #_ #_ #t h1 h2 h3 = h in
-    lem_if_fv_in_env g e1 e2 e3;
-    lem_exp_to_fstar g e1 tbool h1;
-    lem_exp_to_fstar g e2 t h2;
-    lem_exp_to_fstar g e3 t h3;
-    let fs_e1 = (exp_to_fstar g e1 tbool h1) in
-    let fs_e2 = (exp_to_fstar g e2 t h2) in
-    let fs_e3 = (exp_to_fstar g e3 t h3) in
-    equiv_if g t fs_e1 fs_e2 fs_e3 e1 e2 e3
-  | EFst e12 ->
-    let TyFst #_ #_ #t1 #t2 h1 = h in
-    lem_fst_fv_in_env g e12;
-    lem_exp_to_fstar g e12 (t1 ^* t2) h1;
-    let fs_e12 = (exp_to_fstar g e12 (t1 ^* t2) h1) in
-    equiv_pair_fst_app g t1 t2 fs_e12 e12
-  | ESnd e12 ->
-    let TySnd #_ #_ #t1 #t2 h1 = h in
-    lem_snd_fv_in_env g e12;
-    lem_exp_to_fstar g e12 (t1 ^* t2) h1;
-    let fs_e12 = (exp_to_fstar g e12 (t1 ^* t2) h1) in
-    equiv_pair_snd_app g t1 t2 fs_e12 e12
-  | EApp e1 e2 ->
-    let TyApp #_ #_ #_ #t1 #t2 h1 h2 = h in
-    lem_app_fv_in_env g e1 e2;
-    lem_exp_to_fstar g e1 (t1 ^-> t2) h1;
-    lem_exp_to_fstar g e2 t1 h2;
-    let fs_e1 = (exp_to_fstar g e1 (t1 ^-> t2) h1) in
-    let fs_e2 = (exp_to_fstar g e2 t1 h2) in
-    equiv_app g t1 t2 fs_e1 fs_e2 e1 e2
-  | ELam body ->
-    let TyLam #_ #body #t1 #t2 hbody = h in
-    lem_lam_fv_in_env g body t1;
-    lem_exp_to_fstar (extend t1 g) body t2 hbody;
-    assert (equiv t2 (exp_to_fstar (extend t1 g) body t2 hbody) body);
-    assert (forall b (s:gsub (extend t1 g) b) (fsG:eval_env (extend t1 g)). fsG ∽ s ==> t2 ⦂ ((exp_to_fstar (extend t1 g) body t2 hbody) fsG, gsubst s body));
-    let g' = extend t1 g in
-    introduce forall b (s:gsub g b) (fsG:eval_env g). fsG ∽ s ==> (t1 ^-> t2) ⦂ ((fun x -> exp_to_fstar (extend t1 g) body t2 hbody (stack fsG x)), gsubst s (ELam body)) with
-      begin
-      let f : (get_Type t1) -> (get_Type t2) = (fun x -> exp_to_fstar (extend t1 g) body t2 hbody (stack fsG x)) in
-      let body' = subst (sub_elam s) body in
-      assert (gsubst s (ELam body) == ELam body');
-      introduce  fsG ∽ s ==> (t1 ^-> t2) ⦂ (f, ELam body') with _.
-        begin
-        introduce forall (e':closed_exp). steps (ELam body') e' /\ irred e' ==> (t1 ^-> t2) ∋ (f, e') with
-          begin
-          introduce _ ==> (t1 ^-> t2) ∋ (f, e') with h.
-            begin
-            lem_value_is_irred (ELam body');
-            lem_steps_irred_e_irred_e'_implies_e_e' (ELam body') e';
-            assert ((ELam body') == e');
-            let QArr #s1 #s2 r1 r2 = get_rel (t1 ^-> t2) in
-            introduce forall (v:value) (fs_v:get_Type t1). t1 ∋ (fs_v, v) ==> t2 ⦂ (f fs_v, subst_beta v body') with
-              begin
-              introduce  t1 ∋ (fs_v, v) ==> _ with _.
-                begin
-                let s' = gsub_extend s t1 v in
-                let fsG' = stack fsG fs_v in
-                lem_substitution s t1 v body;
-                assert (t2 ⦂ (f fs_v, gsubst s' body))
-                end
-              end;
-              assert ((t1 ^-> t2) ∋ (f, gsubst s (ELam body)));
-              lem_values_are_expressions (t1 ^-> t2) f (gsubst s (ELam body));
-              assert ((t1 ^-> t2) ⦂ (f, gsubst s (ELam body)))
-            end
-          end
-        end
-      end
-#pop-options
 
 val lem_bt_ctx i ct : Lemma (
   let (| e, h |) = ct in
-  pack i.comp_ct ∋ (backtranslate_ctx #i ct, e)
+    (comp_int i).ct ∋ (backtranslate_ctx #i ct, e)
   )
 let lem_bt_ctx i ct =
   let (| e, h |) = ct in
   lem_value_is_closed e;
   lem_closed_is_no_fv e;
   assert (fv_in_env empty e);
-  lem_exp_to_fstar empty e (comp_int i).ct h;
-  equiv_closed_terms #(comp_int i).ct (exp_to_fstar empty e (comp_int i).ct h empty_eval) e;
+  lem_backtranslate empty e (comp_int i).ct h;
+  equiv_closed_terms #(comp_int i).ct (backtranslate empty e (comp_int i).ct h empty_eval) e;
   // t : (bt e, e) and the fact that e is a value implies they are in the value relation (the statement of the lemma)
   ()
 
 (** This variant implies RrHP **)
-let rrhp_1 (#i:intS) (ps:progS i) =
-  forall ct. behS (linkS ps (backtranslate_ctx ct)) `rel_behs` behT (linkT (compile_prog ps) ct)
+let rrhp_1 (#i:intS) =
+  forall (ps:progS i).
+    forall ct. behS (linkS ps (backtranslate_ctx ct)) `rel_behs` behT (linkT (compile_prog ps) ct)
 
-let proof_rrhp_1 i ps : Lemma (rrhp_1 #i ps) =
-  introduce forall ct. behS (linkS ps (backtranslate_ctx ct)) `rel_behs` behT (linkT (compile_prog ps) ct) with begin
-    let t : qType = pack (i.comp_ct) in
-    let pt : exp = (dsnd ps).e in
-    let pt : progT (comp_int i) = pt in
+let proof_rrhp_1 i : Lemma (rrhp_1 #i) =
+  introduce forall ps ct. behS (linkS ps (backtranslate_ctx ct)) `rel_behs` behT (linkT (compile_prog ps) ct) with begin
+    let t : qType = i.ct in
+    let pt : progT (comp_int i) = compile_prog ps in
     let ws : wholeS = (dfst ps) (backtranslate_ctx ct) in
     let (| e, h |) = ct in
     let wt : exp = EApp pt e in
     let wt : wholeT = wt in
-    (dsnd ps).equiv_proof ();
+    compile_equiv (dsnd ps);
     let ps' = dfst ps in
-    lemma_compile_closed_in_equiv_rel ps' #(dsnd ps);
+    compile_closed_equiv (dsnd ps);
     assert ((t ^-> tbool) ⦂ (ps', pt));
-    lemma_compile_closed_arrow_is_elam #_ #_ #i.comp_ct ps' #(dsnd ps);
+    lemma_compile_closed_arrow_is_elam (dsnd ps);
     assert (ELam? pt /\ is_closed pt /\ irred pt);
     eliminate forall (e':closed_exp). steps pt e' ==> irred e' ==>  (t ^-> tbool) ∋ (ps', e') with pt;
     assert ((t ^-> tbool) ∋ (ps', pt));
