rupicola/stlc/Metaprogram.fst
@@ -1,0 +1,121 @@
+module Metaprogram
+
+open FStar.Tactics
+open FStar.Tactics.Typeclasses
+
+open QTyp
+open QExp
+
+(** fs_hd' works better with typeclass resolution than fs_hd **)
+[@"opaque_to_smt"] (** not sure if it is the right pragma to prevent F* unfolding get_v' during type class resolution **)
+val hd' : #g:typ_env -> #t:qType -> eval_env (extend t g) -> a:Type{a == get_Type t} -> a
+let hd' #g fsG a =
+  hd fsG
+
+class quotable_typ (s:Type) = {
+  [@@@no_method] q : type_quotation s;
+}
+
+let pack #s (c:quotable_typ s) : qType = (| s, c.q |)
+
+instance quotable_typ_unit : quotable_typ unit = { q = QUnit }
+instance quotable_typ_bool : quotable_typ bool = { q = QBool }
+instance quotable_typ_arrow
+  (s1:Type)
+  (s2:Type)
+  {| c1:quotable_typ s1 |}
+  {| c2:quotable_typ s2 |} :
+  quotable_typ (s1 -> s2) = { q = QArr c1.q c2.q }
+instance quotable_typ_pair (s1:Type) (s2:Type) {| c1:quotable_typ s1 |} {| c2:quotable_typ s2 |} : quotable_typ (s1 & s2) = { q = QPair c1.q c2.q }
+
+class quotable_exp (#a:Type0) {| ca: quotable_typ a |} (g:typ_env) (s:eval_env g -> a) = { (** using fs_oexp g (pack ca) complicates the instances of the type class **)
+  [@@@no_method] q : exp_quotation #(pack ca) g s;
+}
+
+unfold let quotable (#a:Type0) {| ca: quotable_typ a |} (s:a) =
+  quotable_exp #a empty (fun _ -> s)
+
+instance quotable_tt g : quotable_exp #unit #solve g (fun _ -> ()) = {
+  q = Qtt;
+}
+
+instance quotable_true g : quotable_exp #bool #solve g (fun _ -> true) = {
+  q = QTrue;
+}
+
+instance quotable_false g : quotable_exp #bool #solve g (fun _ -> false) = {
+  q = QFalse;
+}
+
+instance quotable_var0
+  (g:typ_env)
+  (a:Type)
+  {| qa:quotable_typ a |}
+  : quotable_exp #a #qa (extend (pack qa) g) (fun fsG -> hd' fsG a) = {
+    q = magic (); //QVar0;
+}
+
+let test1_var : quotable_exp (extend qUnit empty) (fun fsG -> hd fsG) = solve
+
+instance quotable_var1
+  (g:typ_env)
+  (a:Type)
+  (b:Type)
+  {| qa:quotable_typ a |}
+  {| qb:quotable_typ b |}
+  : quotable_exp #a #qa (extend (pack qb) (extend (pack qa) g))
+    (fun fsG -> hd' (tail fsG) a) = {
+    q = magic (); // QVar1;
+}
+
+instance quotable_var2
+  (g:typ_env)
+  (a:Type)
+  (b:Type)
+  (c:Type)
+  {| qa:quotable_typ a |}
+  {| qb:quotable_typ b |}
+  {| qc:quotable_typ c |}
+  : quotable_exp #a #qa (extend (pack qc) (extend (pack qb) (extend (pack qa) g)))
+    (fun fsG -> hd' (tail (tail fsG)) a) = {
+    q = magic (); // QVar2;
+}
+
+(**
+let test2_var : quotable_exp (extend qUnit (extend qUnit empty)) (fun fsG -> hd' (tail fsG) unit) =
+  solve
+
+let test3_var : compile_exp (extend tunit (extend tunit (extend tunit empty))) (fun fsG -> hd' (tail (tail fsG)) unit) =
+  solve
+**)
+
+instance quotable_lambda
+  g
+  (a:Type) {| qa: quotable_typ a |}
+  (b:Type) {| qb: quotable_typ b |}
+  (f:eval_env g -> a -> b)
+  {| cf: quotable_exp #b #qb (extend (pack qa) g) (fun fsG -> f (tail #(pack qa) fsG) (hd' fsG a)) |}
+  : quotable_exp g f = {
+  q = magic ();
+}
+
+instance quotable_app
+  g
+  (a:Type) {| qa: quotable_typ a |}
+  (b:Type) {| qb: quotable_typ b |}
+  (f:eval_env g -> a -> b) {| qf: quotable_exp #_ #solve g f |}
+  (x:eval_env g -> a)     {| qx: quotable_exp #_ #qa g x |}
+  : quotable_exp #_ #qb g (fun fsG -> (f fsG) (x fsG)) = {
+  q = QApp qf.q qx.q;
+}
+
+instance quotable_if
+  g
+  (co:eval_env g -> bool)  {| qco: quotable_exp #_ #solve g co |}
+
+  (a:Type) {| qa: quotable_typ a |}
+  (th:eval_env g -> a)     {| qth: quotable_exp #_ #qa g th |}
+  (el:eval_env g -> a)     {| qel: quotable_exp #_ #qa g el |}
+  : quotable_exp #_ #qa g (fun fsG -> if co fsG then th fsG else el fsG) = {
+  q = QIf qco.q qth.q qel.q
+}
